Add support for existential variable to "ensatz"

theories/nsatz/ENsatzTactic.v
@@ -10,9 +10,10 @@
 
 (*
  Tactic ensatz: proofs of polynomials equalities in an integral domain
- (commutative ring without zero divisor) with existential quantifier.
+ (commutative ring without zero divisor) with existential quantifier or
+ existential variables.
 
- Examples: see test-suite/success/ENsatz.v
+ Examples: see test-suite/success/ENsatz.v and test-suite/success/EENsatz.v
 
 *)
 
@@ -27,163 +28,169 @@ Section ensatz.
 
   Context {R:Type}`{Rid:Integral_domain R}.
 
-  Local Fixpoint LTType (A : Type) (l : list A) {struct l} : Type :=
+  Local Fixpoint LTType {A: Type} (B : Type) (l : list A) {struct l} : Type :=
     match l with
     | nil => unit
-    |  _ :: l0 =>  (R * LTType A l0)%type
+    |  _ :: l0 =>  (B * LTType B l0)%type
     end.
 
   Local Fixpoint Cond0
     (A : Type) (Interp : A -> R) (l : list A) {struct l} : (LTType A l -> R) :=
     match l return (LTType A l -> R) with
-    | nil => (fun _ => ring0)
-    | a :: l0 => (fun n => add (mul (fst n) (Interp a))
-                        (Cond0 A Interp l0 (snd n)))
+    | nil => fun _ => ring0
+    | a :: l0 =>
+        fun n => add (mul (Interp (fst n)) (Interp a))
+                   (Cond0 A Interp l0 (snd n))
     end.
 
-  Local Definition mk_Cond0 (A : Type) (Interp : A -> R) (l : list A) (v : R) :=
-    exists n, (v == Cond0 A Interp l n).
-
-  Local Fixpoint ring0_tuple (A :Type) (l: list A) : LTType A l :=
-    match l return (LTType A l) with
+  Local Fixpoint ring0_tuple (A :Type) (l: list A) : LTType R l :=
+    match l return (LTType R l) with
     | nil => tt
     | a :: q => (ring0, ring0_tuple A q)
     end.
 
   Local Fixpoint add_coef
-    (A : Type)
-    (Interp : A -> R)
-    (l: list A)  (a : list A)
-    (c : R) {struct l} : (LTType A l -> LTType A l) :=
-    match l, a return  (LTType A l -> LTType A l) with
+    (l: list PolZ)  (a : list PolZ) (c : PolZ)
+    {struct l} : (LTType PolZ l -> LTType PolZ l) :=
+    match l, a return  (LTType PolZ l -> LTType PolZ l) with
     | nil, _ => (fun _ => tt)
     | _, nil => (fun x => x)
-    | h :: q , hx :: qx =>
-        let coef := c * (Interp hx) in
-        fun x => (coef + fst x, add_coef A Interp q qx c (snd x))
+    | _ :: q , hx :: qx =>
+        let coef := PolZmul c hx in
+        fun x => (PolZadd coef (fst x), add_coef q qx c (snd x))
+    end.
+
+  Local Fixpoint certi_aux
+    (lpe: list PolZ) (lq: list PEZ): LTType PolZ lpe :=
+    match lpe, lq return (LTType PolZ lpe) with
+    |  nil, _ => tt
+    |  h::q, nil=> (P0Z, certi_aux q lq)
+    |  h1::q1, h2::q2=> (norm h2, certi_aux q1 q2 )
+    end.
+
+  Local Fixpoint certi
+    (lla : list (list PEZ)) (lpe: list PolZ) (lq: list PEZ) : LTType PolZ lpe :=
+    match lla return (LTType PolZ lpe) with
+    | nil => certi_aux lpe lq
+    | h::q =>
+        let l := certi q ((mult_l h lpe) :: lpe) lq in
+        add_coef lpe (map norm h) (fst l) (snd l)
     end.
 
   Local Definition PhiR := @PhiR R ring0 ring1 add mul opp.
 
   Local Lemma factories_compute_list :
     forall lla l lpe lq,
-      mk_Cond0 PolZ (PhiR l) lpe
-        (PhiR l (mult_l lq (compute_list lla lpe))).
+      PhiR l (mult_l lq (compute_list lla lpe)) ==
+        Cond0 PolZ (PhiR l) lpe (certi lla lpe lq).
   Proof.
-    unfold mk_Cond0.
     induction lla.
     - induction lpe.
-      + destruct lq;simpl;exists tt; reflexivity.
-      + intros;simpl.
-        destruct lq.
-        * simpl.
-          simpl in IHlpe.
-          specialize (IHlpe nil) as (x,H).
-          exists (ring0,x).
+      + destruct lq;simpl; reflexivity.
+      + destruct lq;simpl; simpl in IHlpe.
+        * specialize (IHlpe nil) as H.
           rewrite <- H.
           cring.
-        * simpl.
-          simpl in IHlpe.
-          specialize (IHlpe lq) as (x, H).
-          exists (PhiR l (norm p),x);unfold PhiR.
+        * specialize (IHlpe lq) as H.
+          unfold PhiR.
           rewrite  PolZadd_correct.
           rewrite PolZmul_correct.
           rewrite <- H.
           cring.
     - intros. simpl.
-      specialize (IHlla l (mult_l a lpe :: lpe) lq).
-      destruct IHlla.
+      specialize (IHlla l (mult_l a lpe :: lpe) lq) as H.
       simpl in H.
-      exists (add_coef PolZ (PhiR l) lpe (map norm a) (fst x) (snd x)).
-      unfold PhiR. rewrite H. clear H.
-      destruct x.
-      simpl.
-      generalize dependent lpe.
+      remember (fst (certi lla (mult_l a lpe :: lpe) lq)) as r.
+      remember (snd (certi lla (mult_l a lpe :: lpe) lq)) as l0.
+      clear Heql0. clear Heqr.
+      rewrite H. clear H.
+      revert l0; revert lpe.
       induction a.
-      + intros; destruct lpe; cring.
+      + intros;destruct lpe; simpl; cring.
       + intros.
         destruct lpe;[ cring |].
-        simpl. unfold PhiR.
-        rewrite PolZadd_correct.
-        rewrite PolZmul_correct.
-        specialize (IHa lpe (snd l0)).
+        simpl.
+        specialize (IHa lpe).
         rewrite <- IHa.
+        repeat setoid_rewrite PolZadd_correct.
+        repeat setoid_rewrite PolZmul_correct.
         cring.
   Qed.
 
   (* The type of the existential *)
 
-  Local Fixpoint LTEType (A : Type) (l : list (bool * A)) {struct l} : Type :=
+  Local Fixpoint LTEType
+    {A : Type} (B: Type) (l : list (bool * A)) {struct l} : Type :=
     match l with
     | nil => unit
-    | (true, _) :: l0 =>  (R * LTEType A l0)%type
-    | (false,_)  :: l0 =>  LTEType A l0
+    | (true, _) :: l0 =>  (B * LTEType B l0)%type
+    | (false, _) :: l0 =>  LTEType B l0
     end.
 
   Local Fixpoint btype_to_ftype
-    (A B : Type)
-    (norm :  A -> B)
-    (l: list (bool*A)) {struct l} : (LTType B (map norm (map snd l)) -> LTEType A l) :=
-    match l return  (LTType B (map norm (map snd l)) -> LTEType A l) with
+    (A B : Type) (norm :  A -> B) (l: list (bool*A))
+    {struct l} : (LTType B (map norm (map snd l)) -> LTEType B l) :=
+    match l return  (LTType B (map norm (map snd l)) -> LTEType B l) with
     | nil => fun _ => tt
-    | (true,a) :: q =>  fun x => (fst x, btype_to_ftype A B norm  q (snd x))
-    | (false,a) :: q =>  fun x => (btype_to_ftype A B norm q (snd x))
+    | (true, _) :: q =>  fun x => (fst x, btype_to_ftype A B norm  q (snd x))
+    | (false, _) :: q =>  fun x => (btype_to_ftype A B norm q (snd x))
     end.
+
+  Local Definition cert (lpe: list (prod bool PEZ)) lci lq:=
+    let p := certi lci (map norm (map snd lpe)) lq in
+    btype_to_ftype PEZ PolZ norm lpe p.
 
   (* For the assumptions *)
 
-  Local Fixpoint mk_HCond0 (A : Type) (Interp : A -> R) (l : list (bool * A)) {struct l} : Prop :=
+  Local Fixpoint mk_HCond0
+    {A : Type} (Interp : A -> R) (l : list (bool * A)) {struct l} : Prop :=
     match l with
     | nil => True
-    | (true, a) :: l0 => (mk_HCond0 A Interp l0)
-    | (false, a) :: l0 => ((Interp a) == 0) /\ (mk_HCond0 A Interp l0)
+    | (true, a) :: l0 => (mk_HCond0 Interp l0)
+    | (false, a) :: l0 => ((Interp a) == 0) /\ (mk_HCond0 Interp l0)
     end.
 
   (* For the conclusion *)
 
-  Local Fixpoint GCond0 (A : Type) (Interp : A -> R) (l : list (bool * A))
-    {struct l} : (LTEType A l -> R) :=
-    match l return (LTEType A l -> R) with
+  Local Fixpoint GCond0
+    {A B : Type} (Interp : A -> R) (Interp' : B -> R) (l : list (bool * A))
+    {struct l} : (LTEType B l -> R) :=
+    match l return (LTEType B l -> R) with
     | nil => (fun _ => ring0)
-    | (true, a) :: l0 => (fun n => add (mul (fst n) (Interp a))
-                                (GCond0 A Interp l0 (snd n)))
-    | (false, a) :: l0 => GCond0 A Interp l0
+    | (true, a) :: l0 => (fun n => add (mul (Interp' (fst n)) (Interp a))
+                                (GCond0 Interp Interp' l0 (snd n)))
+    | (false, a) :: l0 => GCond0 Interp Interp' l0
     end.
 
-  Local Definition mk_GCond0 (A : Type) (Interp : A -> R) (l : list (bool * A)) (v : R) :=
-    exists n, (v == GCond0 A Interp l n).
-
-  Local Lemma check_correct_exists :
+  Local Lemma check_correct:
     forall l lpe qe lci lq ,
       check (map snd lpe) qe (lci,lq) = true ->
-      mk_HCond0 PEZ (PEevalR l) lpe ->
-      mk_GCond0 PEZ (PEevalR l) lpe (PEevalR l qe).
+      mk_HCond0 (PEevalR l) lpe ->
+      (PEevalR l qe) == GCond0 (PEevalR l) (PhiR l) lpe (cert lpe lci lq).
   Proof.
+    unfold cert.
     unfold check;intros l lpe qe lla lq H2 H1.
     apply PolZeq_correct with (l:=l) in H2.
-    unfold mk_GCond0.
     specialize (factories_compute_list lla l (map norm (map snd lpe)) lq) as H.
-    unfold mk_Cond0 in H. destruct H.
     rewrite H in H2.
     clear H.
-    exists (btype_to_ftype PEZ PolZ norm lpe x).
     rewrite norm_correct.
     rewrite H2.
     clear H2.
+    remember (certi lla (map norm (map snd lpe)) lq) as x eqn: Hx.
+    clear Hx.
     induction lpe.
     - cring.
     - destruct a.
       destruct b.
       + simpl in H1.
-        destruct x.
-        specialize (IHlpe l0 H1).
+        specialize (IHlpe H1 (snd x)).
         simpl.
         rewrite IHlpe.
         rewrite norm_correct.
         reflexivity.
       + destruct H1.
-        destruct x.
-        specialize (IHlpe l0 H0).
+        specialize (IHlpe H0 (snd x)).
         simpl.
         rewrite IHlpe.
         unfold PhiR.
@@ -192,40 +199,32 @@ Section ensatz.
         cring.
   Qed.
 
+  Local Fixpoint inter
+    {A B: Type} (Interp: B -> R) (l: list (bool*A)) {struct l} : (LTEType B l -> LTEType R l) :=
+    match l return (LTEType B l -> LTEType R l) with
+    | nil => fun _ => tt
+    | (true, _) :: q => fun x => (Interp (fst x), inter Interp q (snd x))
+    | (false, _) :: q => fun x => inter Interp q x
+    end.
+
+  Local Lemma check_correct_exists :
+    forall l lpe qe lci lq ,
+      check (map snd lpe) qe (lci,lq) = true ->
+      mk_HCond0 (PEevalR l) lpe ->
+      exists n, ((PEevalR l qe) == GCond0 (PEevalR l) (fun x => x) lpe n).
+  Proof.
+    intros * H1 H2.
+    exists (inter (PhiR l) lpe (cert lpe lci lq)).
+    rewrite (check_correct _ _ _ _ _ H1 H2).
+    remember (cert lpe lci lq) as x eqn: Hx.
+    clear H1 H2 Hx.
+    induction lpe.
+    - reflexivity.
+    - destruct a.
+      destruct b; simpl; rewrite <- IHlpe; reflexivity.
+  Qed.
+
 End ensatz.
-
-Module Mk_exists.
-
-  Local Ltac mk_tuple R l f :=
-    match l with
-    | (?a :: ?h) =>
-        let t := mk_tuple R h f in
-        constr:((t, f a))
-    | (?a1 :: ?a2 :: @nil R) => constr:((f a2,f a1))
-    end.
-
-  Local Ltac destr_tuple R l f :=
-    match goal with
-    | x : (R * ?A)%type |- _ =>
-        let z := fresh "z" in
-        destruct x as [z x];
-        let l := constr:(z :: l) in
-        destr_tuple R l f
-    | x : (unit)%type |- _ =>
-        let l := eval compute in (l) in
-        let t := mk_tuple R l f in
-        exists t
-   end.
-
-  Ltac mk_exists R x f :=
-    match goal with
-    | x : (R * unit)%type |- _ =>
-        let z := fresh "z" in
-        destruct x as [z x]; exists (f z)
-    | x : (R * ?A)%type |- _ => destr_tuple R constr:(@nil R) f
-    end.
-
-End Mk_exists.
 
 Module Mk_pl.
 
@@ -252,108 +251,25 @@ Module Mk_pl.
 
 End Mk_pl.
 
-Local Ltac ensatz_solve cr R p2 lp2 n fv info :=
-  let p21 := fresh "p21" in
-  let lp21 := fresh "lp21" in
-  let n21 := fresh "n21" in
-  let lv := fresh "lv" in
-  set (p21:=p2); set (lp21:=lp2); set (n21:= n); set(lv := fv);
-  (*We want r to be 1, so we set radicalmax to 1*)
-  NsatzTactic.nsatz_call 1%N info 0%Z p2 lp2
-    ltac:(fun c r lq lci =>
-            let Hg := fresh "Hg" in
-            let c21 := fresh "c" in
-            set (c21 := c);
-            let p211 := constr: (PEmul c p21) in
-            (*If c is not 1/-1, this assert should fail*)
-            assert (Hg:check lp21 p211 (lci,lq) = true);
-            [vm_compute; reflexivity |];
-            let pl := Mk_pl.mk_pl lp21 n in
-            assert (Hg2: mk_HCond0 PEZ (PEevalR lv) pl);
-            [repeat (split;[assumption|idtac]); exact I|];
-            generalize (@check_correct_exists
-                          _ _ _ _ _ _ _ _ _ _ _
-                          lv pl p211 lci lq Hg Hg2);
-            unfold mk_GCond0;
-            let x := fresh "x" in
-            let H1 := fresh "H" in
-            intros [x H1];
-            cbv delta [LTEType]
-              iota beta match in x;
-            match c with
-            | PEc((-1)%Z) => Mk_exists.mk_exists R x constr:(fun x:R => -x);
-                         symmetry in H1
-            | PEc(1%Z) => Mk_exists.mk_exists R x constr:(fun x:R => x)
-            end;
-            cbv delta [PEevalR GCond0
-                         Ring_polynom.PEeval
-                         gen_phiZ gen_phiPOS
-                         InitialRing.gen_phiZ
-                         InitialRing.gen_phiPOS
-                         BinList.nth
-                         jump nth lv p21 fst snd hd]
-              iota beta match in H1;
-              repeat unfold snd;
-              repeat unfold fst;
-              apply NsatzTactic.psos_r1b;
-              NsatzTactic.equalities_to_goal cr;
-              intros <-; cring ).
+Section poly_sort.
+  Context {T:Type}.
+  Context (equal : T -> T -> comparison).
 
-Module Reifi.
-
-  Inductive Var {A: Type}: Type :=
-  | mRef: A -> Var
-  | fstVar :forall B,  @Var (A*B) -> @Var A
-  | sndVar : forall B, @Var (B*A) -> @Var A.
-
-  Local Ltac reify_evar_aux term :=
-    match term with
-    | (fun e => fst (@?P e)) =>
-        let term' := reify_evar_aux P in
-        constr:(fun x => @fstVar _ _ (term' x))
-    | (fun e => snd (@?P e)) =>
-        let term' := reify_evar_aux P in
-        constr:(fun x => @sndVar _ _ (term' x))
-    | (fun e:?T => e) => constr:(fun e :T => mRef e)
-    end.
-
-  Inductive MPoly {R: Type}: Type:=
-  | Poly : MPoly -> (PExpr Z) -> @Var R -> MPoly
+  Inductive MPoly : Type:=
+  | Poly : MPoly -> (PExpr Z) -> T -> MPoly
   | Pc : (PExpr Z) -> MPoly.
 
-  Local Ltac reify_evar R term :=
-    match term with
-    | (fun e => fst _) =>
-        let term' := reify_evar_aux term in
-        constr:(fun e' => @Poly R (@Pc R (PEc 0%Z)) (PEc 1%Z) (term' e'))
-    | (fun e => snd _) =>
-        let term' := reify_evar_aux term in
-        constr:(fun e' => @Poly R (@Pc R (PEc 0%Z)) (PEc 1%Z) (term' e'))
-    | (fun e:?T => e) =>  constr:(fun e':T => @Poly T (@Pc T (PEc 0%Z)) (PEc 1%Z) (mRef e'))
-    end.
-
-  Local Fixpoint mult_mpoly {A: Type} (c : PExpr Z) (p : @MPoly A) : @MPoly A :=
+  Local Fixpoint mult_mpoly (c : PExpr Z) (p : MPoly) : MPoly :=
     match p with
     | Pc e => Pc (PEmul e c)
     | Poly p e v => Poly (mult_mpoly c p) (PEmul e c) v
     end.
 
-  Local Fixpoint equal {A1 A2: Type} (v1 : @Var A1) (v2 : @Var A2): comparison :=
-    match v1, v2 with
-    | mRef _, mRef _ => Eq
-    | fstVar _ v1, fstVar _ v2 => equal v1 v2
-    | sndVar _ v1, sndVar _ v2 => equal v1 v2
-    | fstVar _ _, sndVar _ _ => Gt
-    | sndVar _ _, fstVar _ _ => Lt
-    | _, mRef _ => Gt
-    | mRef _, _ => Lt
-    end.
-
-  Inductive Monom {R: Type}: Type:=
-  | Mon : (PExpr Z) -> @Var R -> Monom
+  Inductive Monom : Type:=
+  | Mon : (PExpr Z) -> T -> Monom
   | Monc : (PExpr Z) -> Monom.
 
-  Local Fixpoint add_monom_poly {A: Type} (p: @MPoly A) (m: @Monom A) :=
+  Local Fixpoint add_monom_poly (p: MPoly) (m: Monom) :=
     match p with
     | Pc e1 =>
         match m with
@@ -372,92 +288,446 @@ Module Reifi.
         end
     end.
 
-  Local Fixpoint add_mpoly {A: Type} (p1 p2 : @MPoly A) : @MPoly A :=
+  Local Fixpoint add_mpoly (p1 p2 : MPoly) : MPoly :=
     match p1 with
     | Pc e1 => add_monom_poly p2 (Monc e1)
     | Poly p1' e1 v1 => add_mpoly p1' (add_monom_poly p2 (Mon e1 v1))
     end.
 
-  Local Fixpoint opp_mpoly {A: Type} (p: @MPoly A) : @MPoly A :=
+  Local Fixpoint opp_mpoly (p: MPoly) : MPoly :=
     match p with
     | Pc e => Pc (PEopp e)
     | Poly p e v => Poly (opp_mpoly p) (PEopp e) v
     end.
 
-  Local Ltac reify R Tring lvar term:=
-    match open_constr:((Tring, term)) with
-    | (Ring (T:=?R) (add:=?add) (mul:=?mul) (sub:=?sub),
-        (fun e1 => ?op (@?E1 e1) (@?E2 e1))) =>
-        let _ := match goal with _ => convert add op end in
-        let E1' := reify R Tring lvar E1 in
-        let E2' := reify R Tring lvar E2 in
-        constr:(fun x => add_mpoly (E1' x) (E2' x))
-    | (Ring (T:=?R) (add:=?add) (mul:=?mul) (sub:=?sub),
-        (fun e1 => ?op (@?E1 e1) (@?E2 e1))) =>
-        let _ := match goal with _ => convert sub op end in
-        let E1' := reify R Tring lvar E1 in
-        let E2' := reify R Tring lvar E2 in
-        constr:(fun x => add_mpoly (E1' x) (opp_mpoly (E2' x)))
-    | (Ring (T:=?R) (ring0:=?ring0) (ring1:=?ring1)
-         (add:=?add) (mul:=?mul) (sub:=?sub) (opp:=?opp),
-        (fun e1 => ?op ?E (@?E1 e1))) =>
-        let _ := match goal with _ => convert mul op end in
-        let E1' := reify R Tring lvar E1 in
-        let E' := reify_term R ring0 ring1 add mul sub opp lvar E in
-        constr:(fun x => mult_mpoly E' (E1' x))
-    | (Ring (T:=?R) (ring0:=?ring0) (ring1:=?ring1)
-         (add:=?add) (mul:=?mul) (sub:=?sub) (opp:=?opp),
-        (fun e1 => ?op (@?E1 e1) ?E)) =>
-        let _ := match goal with _ => convert mul op end in
-        let E1' := reify R Tring lvar E1 in
-        let E' := reify_term R ring0 ring1 add mul sub opp lvar E in
-        constr:(fun x => mult_mpoly E' (E1' x))
-    | (_, (fun e => @?E e)) => reify_evar R E
-    | (Ring (T:=?R) (opp:=?opp), (fun e => ?op (@?E e))) =>
-        let _ := match goal with _ => convert opp op end in
-        let E' := reify_evar R E in
-        constr:(fun x => opp_mpoly (E' x))
-    | (Ring (T:=?R) (ring0:=?ring0) (ring1:=?ring1)
-         (add:=?add) (mul:=?mul) (sub:=?sub) (opp:=?opp),
-        (fun _:?T => ?E)) =>
-        let E' := reify_term R ring0 ring1 add mul sub opp lvar E in
-        constr:(fun _:T => @Pc R E')
-    end.
-
-  Local Fixpoint get_coef {A:Type} (p: @MPoly A) :=
+  Local Fixpoint get_coef (p: MPoly) :=
     match p with
     | Pc e => e :: nil
     | Poly p e v => e :: get_coef p
     end.
 
-  Local Definition coef {A R:Type} (p: A -> @MPoly R) :=
-    fun x => get_coef (p x).
+End poly_sort.
 
-  Local Definition merge {A R:Type} (p1 p2: A -> @MPoly R) :=
-    fun x => add_mpoly (p1 x) (opp_mpoly (p2 x)).
+Module Ensatz_solve.
 
-  Ltac reify_goal  :=
-    match goal with
-    | |- @ex _ (fun e1 : _ => @eq ?R (@?P1 e1) (@?P2 e1)) =>
-        let lvar := open_constr:(_ :> list R) in
-        let R_ring := constr:(_ :> Ring (T:=R)) in
-        let Tring := type of R_ring in
-        let xl := reify R Tring lvar P1 in
-        let xr := reify R Tring lvar P2 in
-        let x := eval cbv delta
-                   [merge coef
-                      get_coef
-                      add_mpoly
-                      mult_mpoly
-                      add_monom_poly
-                      equal
-                      opp_mpoly]
-                   beta iota in (coef (merge xr xl))
-          in
-          constr:((lvar,x))
+  Local Ltac mk_tuple R l f :=
+    match l with
+    | (?a :: ?h) =>
+        let t := mk_tuple R h f in
+        constr:((t, f a))
+    | (?a1 :: ?a2 :: @nil R) => constr:((f a2,f a1))
     end.
 
-End Reifi.
+  Local Ltac destr_tuple R l f :=
+    match goal with
+    | x : (R * ?A)%type |- _ =>
+        let z := fresh "z" in
+        destruct x as [z x];
+        let l := constr:(z :: l) in
+        destr_tuple R l f
+    | x : (unit)%type |- _ =>
+        let l := eval compute in (l) in
+        let t := mk_tuple R l f in
+        exists t
+     end.
+
+  Ltac mk_exists R x f :=
+    match goal with
+    | x : (R * unit)%type |- _ =>
+        let z := fresh "z" in
+        destruct x as [z x]; exists (f z)
+    | x : (R * ?A)%type |- _ =>
+        destr_tuple R constr:(@nil R) f
+    end.
+
+  Ltac ensatz_solve cr R p2 lp2 n fv info :=
+    let p21 := fresh "p21" in
+    let lp21 := fresh "lp21" in
+    let n21 := fresh "n21" in
+    let lv := fresh "lv" in
+    set (p21:=p2); set (lp21:=lp2); set (n21:= n); set(lv := fv);
+    (*We want r to be 1, so we set radicalmax to 1*)
+    NsatzTactic.nsatz_call 1%N info 0%Z p2 lp2
+      ltac:(fun c r lq lci =>
+              let Hg := fresh "Hg" in
+              let c21 := fresh "c" in
+              set (c21 := c);
+              let p211 := constr: (PEmul c p21) in
+              let pl := Mk_pl.mk_pl lp21 n in
+              (*If c is not 1/-1, this assert should fail*)
+              assert (Hg:check lp21 p211 (lci,lq) = true);
+              [vm_compute; reflexivity |];
+              assert (Hg2: mk_HCond0 (PEevalR lv) pl);
+              [repeat (split;[assumption|idtac]); exact I|];
+              generalize (@check_correct_exists
+                            _ _ _ _ _ _ _ _ _ _ _
+                            lv pl p211 lci lq Hg Hg2);
+              let x := fresh "x" in
+              let H1 := fresh "H" in
+              intros [x H1];
+              cbv delta [LTEType] iota beta match in x;
+              match c with
+              | PEc((-1)%Z) => mk_exists R x constr:(fun x:R => -x);
+                              symmetry in H1
+              | PEc(1%Z) => mk_exists R x constr:(fun x:R => x)
+              end;
+              cbv delta [lv p21] in H1;
+              cbv delta
+                [PEevalR
+                   GCond0
+                   Ring_polynom.PEeval
+                   gen_phiZ gen_phiPOS
+                   InitialRing.gen_phiZ
+                   InitialRing.gen_phiPOS
+                   BinList.nth
+                   jump fst snd hd]
+                iota beta match in H1;
+               repeat unfold snd;
+               repeat unfold fst;
+               apply NsatzTactic.psos_r1b;
+               NsatzTactic.equalities_to_goal cr;
+               intros <-; cring
+           ).
+
+  Module Reifi.
+
+    Inductive Var {A: Type}: Type :=
+    | mRef: A -> Var
+    | fstVar : forall B, @Var (A*B) -> @Var A
+    | sndVar : forall B, @Var (B*A) -> @Var A.
+
+    Local Ltac reify_evar_aux term :=
+      match term with
+      | (fun e => fst (@?P e)) =>
+          let term' := reify_evar_aux P in
+          constr:(fun x => @fstVar _ _ (term' x))
+      | (fun e => snd (@?P e)) =>
+          let term' := reify_evar_aux P in
+          constr:(fun x => @sndVar _ _ (term' x))
+      | (fun e:?T => e) => constr:(fun e :T => mRef e)
+      end.
+
+    Local Ltac reify_evar R term :=
+      match term with
+      | (fun e => fst _) =>
+          let term' := reify_evar_aux term in
+          constr:
+            (fun e' =>
+               @Poly (@Var R) (@Pc (@Var R) (PEc 0%Z)) (PEc 1%Z) (term' e'))
+      | (fun e => snd _) =>
+          let term' := reify_evar_aux term in
+          constr:
+            (fun e' =>
+               @Poly (@Var R) (@Pc (@Var R) (PEc 0%Z)) (PEc 1%Z) (term' e'))
+      | (fun e:?T => e) =>
+          constr:
+            (fun e':T =>
+               @Poly (@Var T) (@Pc (@Var T) (PEc 0%Z)) (PEc 1%Z) (mRef e'))
+      end.
+
+    Local Fixpoint equal
+      {A1 A2: Type} (v1 : @Var A1) (v2 : @Var A2): comparison :=
+      match v1, v2 with
+      | mRef _, mRef _ => Eq
+      | fstVar _ v1, fstVar _ v2 => equal v1 v2
+      | sndVar _ v1, sndVar _ v2 => equal v1 v2
+      | fstVar _ _, sndVar _ _ => Gt
+      | sndVar _ _, fstVar _ _ => Lt
+      | _, mRef _ => Gt
+      | mRef _, _ => Lt
+      end.
+
+    Local Definition add_mpoly
+      {A: Type} (p1 p2 : @MPoly (@Var A)) : @MPoly (@Var A):=
+      add_mpoly equal p1 p2.
+
+    Local Ltac reify R Tring lvar term:=
+      match open_constr:((Tring, term)) with
+      | (Ring (T:=?R) (add:=?add) (mul:=?mul) (sub:=?sub),
+          (fun e1 => ?op (@?E1 e1) (@?E2 e1))) =>
+          let _ := match goal with _ => convert add op end in
+          let E1' := reify R Tring lvar E1 in
+          let E2' := reify R Tring lvar E2 in
+          constr:(fun x => add_mpoly (E1' x) (E2' x))
+      | (Ring (T:=?R) (add:=?add) (mul:=?mul) (sub:=?sub),
+          (fun e1 => ?op (@?E1 e1) (@?E2 e1))) =>
+          let _ := match goal with _ => convert sub op end in
+          let E1' := reify R Tring lvar E1 in
+          let E2' := reify R Tring lvar E2 in
+          constr:(fun x => add_mpoly (E1' x) (opp_mpoly (E2' x)))
+      | (Ring (T:=?R) (ring0:=?ring0) (ring1:=?ring1)
+           (add:=?add) (mul:=?mul) (sub:=?sub) (opp:=?opp),
+          (fun e1 => ?op ?E (@?E1 e1))) =>
+          let _ := match goal with _ => convert mul op end in
+          let E1' := reify R Tring lvar E1 in
+          let E' := reify_term R ring0 ring1 add mul sub opp lvar E in
+          constr:(fun x => mult_mpoly E' (E1' x))
+      | (Ring (T:=?R) (ring0:=?ring0) (ring1:=?ring1)
+           (add:=?add) (mul:=?mul) (sub:=?sub) (opp:=?opp),
+          (fun e1 => ?op (@?E1 e1) ?E)) =>
+          let _ := match goal with _ => convert mul op end in
+          let E1' := reify R Tring lvar E1 in
+          let E' := reify_term R ring0 ring1 add mul sub opp lvar E in
+          constr:(fun x => mult_mpoly E' (E1' x))
+      | (_, (fun e => @?E e)) => reify_evar R E
+      | (Ring (T:=?R) (opp:=?opp), (fun e => ?op (@?E e))) =>
+          let _ := match goal with _ => convert opp op end in
+          let E' := reify_evar R E in
+          constr:(fun x => opp_mpoly (E' x))
+      | (Ring (T:=?R) (ring0:=?ring0) (ring1:=?ring1)
+           (add:=?add) (mul:=?mul) (sub:=?sub) (opp:=?opp),
+          (fun _:?T => ?E)) =>
+          let E' := reify_term R ring0 ring1 add mul sub opp lvar E in
+          constr:(fun _:T => @Pc (@Var R) E')
+      end.
+
+    Local Definition coef {A R:Type} (p: A -> @MPoly (@Var R)) :=
+      fun x => get_coef (p x).
+
+    Local Definition merge {A R:Type} (p1 p2: A -> @MPoly (@Var R)) :=
+      fun x => add_mpoly (p1 x) (opp_mpoly (p2 x)).
+
+    Ltac reify_goal  :=
+      match goal with
+      | |- @ex _ (fun e1 : _ => @eq ?R (@?P1 e1) (@?P2 e1)) =>
+          let lvar := open_constr:(_ :> list R) in
+          let R_ring := constr:(_ :> Ring (T:=R)) in
+          let Tring := type of R_ring in
+          let xl := reify R Tring lvar P1 in
+          let xr := reify R Tring lvar P2 in
+          let x :=
+            eval cbv delta
+              [merge
+                 coef
+                 get_coef
+                 add_mpoly
+                 ENsatzTactic.add_mpoly
+                 mult_mpoly
+                 add_monom_poly
+                 equal
+                 opp_mpoly]
+              beta iota in (coef (merge xr xl))
+           in
+           constr:((lvar,x))
+      end.
+
+  End Reifi.
+
+  Ltac hterm R g :=
+    match g with
+    | (exists _: _, _ ) => constr:((@nil R))
+    | ?b1 == ?b2 -> ?g =>
+        let l := hterm R g in
+        constr:((b1 :: l))
+    end.
+
+End Ensatz_solve.
+
+Module Eensatz_solve.
+
+  Local Ltac econstrain_aux R ring0 ring1 add mul opp l lc lv z:=
+    match open_constr:((lc, lv)) with
+    |((?c, ?q1), @cons _ ?v ?q2) =>
+       let c := eval cbv delta [l]in (@PhiR R ring0 ring1 add mul opp l c) in
+       let c :=
+         eval cbv delta
+           [PhiR
+              NsatzTactic.PhiR
+              Pphi
+              gen_phiZ
+              gen_phiPOS
+              pow_pos
+              jump hd tl]
+           iota beta match in c
+       in
+       let v := eval cbv delta [l] in (PEevalR l v) in
+       let v :=
+         eval cbv delta
+           [PEevalR
+              GCond0
+              Ring_polynom.PEeval
+              gen_phiZ gen_phiPOS
+              InitialRing.gen_phiZ
+              InitialRing.gen_phiPOS
+              BinList.nth
+              jump tl fst snd hd]
+           iota beta match in v
+       in
+       assert (v = z * c) by reflexivity;
+       econstrain_aux R ring0 ring1 add mul opp l q1 q2 z
+    | (_, _) => idtac
+    end.
+
+  Local Ltac econstrain R l lc lv z :=
+    let R_ring := constr:(_ :> Ring (T:=R)) in
+    let Tring := type of R_ring in
+    lazymatch Tring with
+      | Ring (T:=?R) (ring0:=?ring0) (ring1:=?ring1)
+          (add:=?add) (mul:=?mul) (sub:=?sub) (opp:=?opp) =>
+          econstrain_aux R ring0 ring1 add mul opp l lc lv z
+    end.
+
+  Ltac ensatz_solve R p2 lp2 n fv vs info :=
+    let p21 := fresh "p21" in
+    let lp21 := fresh "lp21" in
+    let lv := fresh "lv" in
+    let lvs := fresh "lvs" in
+    set (p21:=p2);set (lp21:=lp2); set(lv := fv); set (lvs := vs);
+    (*We want r to be 1, so we set radicalmax to 1*)
+    NsatzTactic.nsatz_call 1%N info 0%Z p2 lp2
+      ltac:(fun c r lq lci =>
+              let Hg := fresh "Hg" in
+              let c21 := fresh "c" in
+              let p211 := constr: (PEmul c p21) in
+              let pl := Mk_pl.mk_pl lp21 n in
+              (*If c is not 1/-1, this assert should fail*)
+              assert (Hg:check lp21 p211 (lci,lq) = true);
+              [vm_compute; reflexivity |];
+              assert (Hg2: mk_HCond0 (PEevalR lv) pl);
+              [repeat (split;[assumption|idtac]); exact I|];
+              generalize (@check_correct
+                            _ _ _ _ _ _ _ _ _ _ _
+                            lv pl p211 lci lq Hg Hg2);
+              let Hc := fresh "Hc" in
+              intro Hc;
+              let Cert := fresh "Cert" in
+              let cert := constr: (cert pl lci lq) in
+              set (Cert := cert);
+              specialize (eq_refl Cert);
+              unfold Cert at 2;
+              let HCert := fresh "HCert" in
+              intro HCert;
+              fold Cert in Hc;
+              compute in Cert;
+              let y := eval simpl in (map (PEevalR lv) vs) in
+              let cert := eval cbv delta [Cert] in Cert in
+              match c with
+              | PEc ((-1)%Z) => econstrain R lv cert vs ((-1)%Z);
+                               symmetry in Hc
+              | PEc (1%Z) => econstrain R lv cert vs (1%Z)
+              end;
+              cbv delta [Cert lv p21] in Hc;
+              cbv delta
+                [PEevalR
+                   GCond0
+                   Ring_polynom.PEeval
+                   gen_phiZ gen_phiPOS
+                   InitialRing.gen_phiZ
+                   InitialRing.gen_phiPOS
+                   BinList.nth
+                   jump tl fst snd hd]
+               iota beta match in Hc;
+               cbv delta
+                 [PhiR
+                    NsatzTactic.PhiR
+                    Pphi gen_phiZ
+                    gen_phiPOS
+                    pow_pos
+                    jump hd tl]
+               iota beta match in Hc;
+              apply NsatzTactic.psos_r1b;
+              apply psos_r1 in Hc;
+              rewrite <- Hc;
+              cring
+           ).
+
+  Module Reifi.
+
+    Local Definition add_mpoly (p1 p2 : @MPoly positive) : @MPoly positive:=
+      add_mpoly Pos.compare p1 p2.
+
+    Local Ltac areify R Tring lvar term:=
+      match open_constr:((Tring, term)) with
+      | (Ring
+           (T:=?R) (ring0:=?ring0) (ring1:=?ring1)
+           (add:=?add) (mul:=?mul) (sub:=?sub) (opp:=?opp), ?E) =>
+          let __ := match E with _ => is_ground E end in
+          let E' := reify_term R ring0 ring1 add mul sub opp lvar E in
+          constr:((@Pc positive E'))
+      | (Ring
+           (T:=?R) (ring0:=?ring0) (ring1:=?ring1)
+           (add:=?add) (mul:=?mul) (sub:=?sub) (opp:=?opp), ?E) =>
+          let __ := match E with _ => is_evar E end in
+          let E' := reify_term R ring0 ring1 add mul sub opp lvar E in
+          let n :=
+            match E' with
+            | PEX _ ?n => n
+            end
+          in
+          constr:(@Poly positive (@Pc positive (PEc 0%Z)) (PEc 1%Z) n)
+      | (Ring
+           (T:=?R) (ring0:=?ring0) (ring1:=?ring1)
+           (add:=?add) (mul:=?mul) (sub:=?sub) (opp:=?opp), ?op ?E1 ?E2) =>
+          let _ := match goal with _ => convert mul op end in
+          let _ := match E1 with _ => is_ground E1 end in
+          let _ := match E2 with _ => has_evar E2 end in
+          let E1' := reify_term R ring0 ring1 add mul sub opp lvar E1 in
+          let E2' := areify R Tring lvar E2 in
+          constr:(mult_mpoly E1' E2')
+      | (Ring
+           (T:=?R) (ring0:=?ring0) (ring1:=?ring1)
+           (add:=?add) (mul:=?mul) (sub:=?sub) (opp:=?opp), ?op ?E1 ?E2) =>
+          let _ := match goal with _ => convert mul op end in
+          let _ := match E1 with _ => has_evar E1 end in
+          let _ := match E2 with _ => is_ground E2 end in
+          let E1' := areify R Tring lvar E1 in
+          let E2' := reify_term R ring0 ring1 add mul sub opp lvar E2 in
+          constr:(mult_mpoly E2' E1')
+      | (Ring
+           (T:=?R) (add:=?add) (mul:=?mul) (sub:=?sub)
+           (opp:=?opp), ?op ?E1 ?E2) =>
+          let _ := match goal with _ => convert add op end in
+          let E1' := areify R Tring lvar E1 in
+          let E2' := areify R Tring lvar E2 in
+          constr:(add_mpoly E1' E2')
+      | (Ring (T:=?R) (add:=?add) (mul:=?mul) (sub:=?sub), ?op ?E1 ?E2) =>
+          let _ := match goal with _ => convert sub op end in
+          let E1' := areify R Tring lvar E1 in
+          let E2' := areify R Tring lvar E2 in
+          constr:(add_mpoly E1' (opp_mpoly E2'))
+      | (Ring (T:=?R) (ring0:=?ring0) (ring1:=?ring1)
+           (add:=?add) (mul:=?mul) (sub:=?sub) (opp:=?opp), (?op ?E)) =>
+          let _ := match goal with _ => convert opp op end in
+          let _ := match E with _ => is_evar E end in
+          let E' := reify_term R ring0 ring1 add mul sub opp lvar E in
+          let n := match E' with
+                   | PEX _ ?n => n
+                   end
+          in
+          constr:(opp_mpoly(@Poly positive (@Pc positive (PEc 0%Z)) (PEc 1%Z) n))
+      end.
+
+    Local Fixpoint get_var (p: @MPoly positive) :=
+      match p with
+      | Pc e => nil
+      | Poly p e v => (PEX Z v) :: get_var p
+      end.
+
+    Ltac reify_goal  :=
+      match goal with
+      | |- @eq ?R ?E1 ?E2 =>
+          let lvar := open_constr:(_ :> list R) in
+          let R_ring := constr:(_ :> Ring (T:=R)) in
+          let Tring := type of R_ring in
+          let xl := areify R Tring lvar E1 in
+          let xr := areify R Tring lvar E2 in
+          let poly := eval vm_compute in (add_mpoly xr (opp_mpoly xl)) in
+          let x := eval vm_compute in (get_coef poly) in
+          let v := eval vm_compute in (get_var poly) in
+          constr:((lvar,x, v))
+      end.
+
+  End Reifi.
+
+  Ltac hterm R g :=
+    match g with
+    | ?b1 = ?b2 => constr:((@nil R))
+    | ?b1 == ?b2 -> ?g =>
+        let l := hterm R g in
+        constr:((b1 :: l))
+    end.
+
+End Eensatz_solve.
 
 Local Ltac reify_h lv lb :=
   match lb with
@@ -469,37 +739,65 @@ Local Ltac reify_h lv lb :=
       list_reifyl R_ring lv lb
  end.
 
-Local Ltac hterm R g :=
-    match g with
-    | (exists _: _, _ ) => constr:((@nil R))
-    | ?b1 == ?b2 -> ?g => let l := hterm R g in
-                         constr:((b1 :: l))
-    end.
+Ltac nsatz_guess_domain :=
+  let eq := match goal with
+            | |- @ex _ (fun e1 : _ => ?eq _ _ ) => eq
+            | |- ?eq _ _ => eq
+            end
+  in
+  let di :=
+    lazymatch
+      open_constr:(ltac:(typeclasses eauto):Integral_domain (ring_eq:=eq))
+    with?di => di end
+  in
+  let __ := match di with _ => assert_fails (is_evar di) end in
+  di.
 
 Lemma efactor:
   forall A B P,  (exists x : A * B, P (fst x) (snd x)) -> (exists x : A, exists y: B, P x y).
 Proof.
-  intros A B P [x H].  eauto.
+  intros A B P [x H]. eauto.
 Qed.
 
-Ltac nsatz_guess_domain :=
-  let eq := match goal with | |- @ex _ (fun e1 : _ => ?eq _ _ ) => eq end in
-  let di := lazymatch open_constr:(ltac:(typeclasses eauto):Integral_domain (ring_eq:=eq)) with?di => di end in
-  let __ := match di with _ => assert_fails (is_evar di) end in
-  di.
-
-Local Ltac ensatz_default info :=
+Ltac ensatz_default info :=
   intros;
   repeat apply efactor;
   let di := nsatz_guess_domain in
   let r := lazymatch type of di with Integral_domain(R:=?r) => r end in
   let cr := lazymatch type of di with Integral_domain(Rcr:=?cr) => cr end in
   match goal with
-  | |- @ex _ (fun e1 : _ => @eq ?R (@?P1 e1) (@?P2 e1)) =>
-      match Reifi.reify_goal with
-      | (?lvar, (fun _: _ => ?x)) =>
+  | |- @eq ?R ?E1 ?E2 =>
+      match Eensatz_solve.Reifi.reify_goal with
+      | (?lvar, ?x, ?v) =>
           let b := eval cbv delta [List.last] iota beta match
-                   in (List.last x (PEc 0%Z))
+                       in (List.last x (PEc 0%Z))
+          in
+          let b := constr: (PEopp b) in
+          let l := constr: (List.removelast x) in
+          let n := eval compute in (List.length l) in
+          repeat NsatzTactic.equalities_to_goal cr;
+          match goal with
+            |- ?g =>
+              let lb := Eensatz_solve.hterm R g in
+              intros;
+              match reify_h lvar lb with
+              | (?fv, ?le) =>
+                let l := constr: (List.rev_append le l) in
+                let le := constr: (b :: l) in
+                let lpol := eval compute in le in
+                match lpol with
+                | ?p2::?lp2 => Eensatz_solve.ensatz_solve R p2 lp2 n fv v info
+                | ?g => idtac "polynomial not in the ideal"
+                end
+              end
+            end
+           end
+  | |- @ex _ (fun e1 : _ => @eq ?R (@?P1 e1) (@?P2 e1)) =>
+      match Ensatz_solve.Reifi.reify_goal with
+      | (?lvar, (fun _: _ => ?x)) =>
+          let b :=
+            eval cbv delta [List.last] iota beta match
+                in (List.last x (PEc 0%Z))
           in
           let b := constr: (PEopp b) in
           let l := constr: (List.removelast x) in
@@ -507,7 +805,7 @@ Local Ltac ensatz_default info :=
           repeat NsatzTactic.equalities_to_goal cr;
           match goal with
            |- ?g =>
-             let lb := hterm R g in
+             let lb := Ensatz_solve.hterm R g in
              intros;
              match reify_h lvar lb with
              | (?fv, ?le) =>
@@ -515,13 +813,13 @@ Local Ltac ensatz_default info :=
                 let le := constr: (b :: l) in
                 let lpol := eval compute in le in
                 match lpol with
-                 | ?p2::?lp2 => ensatz_solve cr R p2 lp2 n fv info
+                | ?p2::?lp2 => Ensatz_solve.ensatz_solve cr R p2 lp2 n fv info
                  | ?g => idtac "polynomial not in the ideal"
                  end
              end
         end
     end
-end.
+  end.
 
 Tactic Notation "ensatz" := ensatz_default 1%Z.
 
